IRLemmasAsCR.v
@@ -1402,11 +1402,10 @@ Proof.
   unfoldMC. ring.
 Qed.
 
+
 Notation "¼" := (QposMake xH (xO (xO xH))).
 Notation  "2" := (QposMake (xO xH) xH).
 Require Export CoRN.util.Extract.
-
-(*
 Eval vm_compute in (answer 2 (√(cos ½))).
 Eval vm_compute in (answer 2 (exp (cos (sin (arctan π))))).
 Lemma demo :  √(cos ½) < exp (cos (sin (arctan (π)))).
@@ -1415,4 +1414,3 @@ Proof.
      exists 1%nat.  vm_compute. 
   (* the price we pay is P or not P. actuall it is not a price. robotics*)
 Abort.
-*)
